code/bignum/Hacl.Impl.Exponentiation.fsti
@@ -207,3 +207,40 @@ val lexp_fw_ct:
   -> ctx_len:size_t
   -> k:lexp a_t len ctx_len ->
   lexp_fw_st a_t len ctx_len k
+
+
+inline_for_extraction noextract
+let lexp_double_fw_st (a_t:inttype_a) (len:size_t{v len > 0}) (ctx_len:size_t) (k:lexp a_t len ctx_len) =
+    ctx:lbuffer (uint_t a_t SEC) ctx_len
+  -> a1:lbuffer (uint_t a_t SEC) len
+  -> bLen:size_t
+  -> bBits:size_t{0 < v bBits /\ (v bBits - 1) / bits a_t < v bLen}
+  -> b1:lbuffer (uint_t a_t SEC) bLen
+  -> a2:lbuffer (uint_t a_t SEC) len
+  -> b2:lbuffer (uint_t a_t SEC) bLen
+  -> acc:lbuffer (uint_t a_t SEC) len
+  -> l:size_t{0 < v l /\ v l < bits a_t /\ pow2 (v l) * v len <= max_size_t /\ v l < 32} ->
+  Stack unit
+  (requires fun h ->
+    live h a1 /\ live h b1 /\ live h a2 /\ live h b2 /\ live h acc /\ live h ctx /\
+    B.loc_pairwise_disjoint [ loc a1; loc b1; loc a2; loc b2; loc acc; loc ctx ] /\
+    BD.bn_v h b1 < pow2 (v bBits) /\
+    BD.bn_v h b2 < pow2 (v bBits) /\
+    k.to.linv_ctx (as_seq h ctx) /\
+    k.to.linv (as_seq h a1) /\ k.to.linv (as_seq h a2) /\
+    k.to.linv (as_seq h acc) /\ k.to.refl (as_seq h acc) == k.to.exp.S.one)
+  (ensures  fun h0 _ h1 -> modifies (loc acc) h0 h1 /\
+    k.to.linv (as_seq h1 acc) /\
+    k.to.refl (as_seq h1 acc) ==
+    S.exp_double_fw #k.to.a_spec k.to.exp
+      (k.to.refl (as_seq h0 a1)) (v bBits) (BD.bn_v h0 b1)
+      (k.to.refl (as_seq h0 a2)) (BD.bn_v h0 b2) (v l))
+
+
+inline_for_extraction noextract
+val lexp_double_fw_raw:
+    #a_t:inttype_a
+  -> len:size_t{v len > 0}
+  -> ctx_len:size_t
+  -> k:lexp a_t len ctx_len ->
+  lexp_double_fw_st a_t len ctx_len k
